src/lib/data/Kuiper.Matrix.Vectorized.fsti
@@ -23,5 +23,5 @@ fn gpu_matrix_vec_read
   preserves gm |-> Frac f em
   requires  pure (aligned' 16 (core gm) (cell_of_pos l i j))
   requires  arr |-> s
-  requires  pure (Pulse.Lib.Array.length arr >= chunk et)
+  requires  pure (Pulse.Lib.Array.length arr == chunk et)
   ensures   arr |-> Seq.init_ghost (chunk et) (fun x -> macc em i (j + x))
